Fixed some bugs to now reach the next hurdle

examples/test3debug.v
@@ -1,181 +1,220 @@
-(**************************************************************************)
-(*                                                                        *)
-(*     SMTCoq                                                             *)
-(*     Copyright (C) 2011 - 2021                                          *)
-(*                                                                        *)
-(*     See file "AUTHORS" for the list of authors                         *)
-(*                                                                        *)
-(*   This file is distributed under the terms of the CeCILL-C licence     *)
-(*                                                                        *)
-(**************************************************************************)
-
-
-(* [Require Import SMTCoq.SMTCoq.] loads the SMTCoq library.
-   If you are using native-coq instead of Coq 8.9, replace it with:
-     Require Import SMTCoq.
-   *)
 Add Rec LoadPath "/home/arjun/Desktop/smtcoq/arjunvish-smtcoq-veritAst/smtcoq/src" as SMTCoq.
-
 Require Import SMTCoq.SMTCoq.
 Require Import Bool.
 Require Import Int31.
 Local Open Scope int31_scope.
 
-Section Checker_SmtEx3Debug.
-  Parse_certif_verit t_i3 t_func3 t_atom3 t_form3 root3 used_roots3 trace3 
-  "/home/arjun/Desktop/smtcoq/arjunvish-smtcoq-veritAst/smtcoq/examples/test3.smt2" 
+Section Test3Debug.
+  Parse_certif_verit t_i3 t_func3 t_atom3 t_form3 root3 used_roots3 trace3
+  "/home/arjun/Desktop/smtcoq/arjunvish-smtcoq-veritAst/smtcoq/examples/test3.smt2"
   "/home/arjun/Desktop/smtcoq/arjunvish-smtcoq-veritAst/smtcoq/examples/test3.vtlog".
-  (*
-  Structures_standard.v
-  ---------------------
-  Definition trace (step:Type) := ((list step) * step)%type.
-
-  Trace.v
-  -------
-  Definition _trace_ := Structures.trace step.
-
-  Inductive certif :=
-  | Certif : int -> _trace_ step -> int -> certif.
-  *)
-  Print trace3.
-  
-  (* Components of the certificate *)
   Definition nclauses3 := Eval vm_compute in (match trace3 with Certif a _ _ => a end). (* Size of the state *)
-  Print nclauses3. (* 4 *)
-  Definition c3 := Eval vm_compute in (match trace3 with Certif _ a _ => a end). (* Certificate of type (list step) * step*)
+  Print nclauses3.
+  Definition c3 := Eval vm_compute in (match trace3 with Certif _ a _ => a end). (* Certificate *)
   Print c3.
-  Definition conf3 := Eval vm_compute in (match trace3 with Certif _ _ a => a end). (* Look here in the state for the empty clause *)
-  Print conf3. (* 1 *)
-  Eval vm_compute in List.length (fst c3).
-  (* 13 steps in the certificate *)
-
-  (* Certif after process_proj (from veritAst):
-      (h1, AssumeAST, (cl  ((and  op_0 (not op_0)))), [], [])
-      (t2, AndnAST, (cl  ((and  (and  op_0 (not op_0)) (not (false)))) ((not (and  op_0 (not op_0)))) ((false))), [], [])
-      (t3, Equp2AST, (cl  ((not ((and  op_0 (not op_0)) = (false)))) ((not (and  op_0 (not op_0)))) ((false))), [], [])
-      (t4, ThresoAST, (cl  ((false))), [ h1 t2 t3], [])
-      (t5, FalsAST, (cl  ((not (false)))), [], [])
-      (t6, ResoAST, (cl ), [ t4 t5], [])
-      (x8, AndAST, (cl  ((and  op_0 (not op_0)))), [ t6], [ 0])
-      (x2, AndAST, (cl  (op_0)), [ x8], [ 0])
-      (x3, AndAST, (cl  ((not op_0))), [ x8], [ 1])
-      (x4, Impn1AST, (cl  ((imp  op_0 (false))) (op_0)), [], [])
-      (x5, ResoAST, (cl  ((imp  op_0 (false)))), [ x3 x4], [])
-      (x6, ImpAST, (cl  ((not op_0)) ((false))), [ x5], [])
-      (x7, ResoAST, (cl  ((false))), [ x2 x6], [])
-      (x9, AndAST, (cl  ((not (false)))), [ t6], [ 1])
-      (x10, ResoAST, (cl ), [ x7 x9], [])
-  *)
-
+  Definition conf3 := Eval vm_compute in (match trace3 with Certif _ _ a => a end). (* Look here in the state for the empty clause*)
+  Print conf3.
+  Eval vm_compute in List.length (fst c3). (* No. of steps in certificate *)
   (* Sanity check that atoms and formulas are well-typed. Must return true *)
   Eval vm_compute in (Form.check_form t_form3 && Atom.check_atom t_atom3 && Atom.wt t_i3 t_func3 t_atom3).
 
 
   (* States from c3 *)
-  
+
   (* Start state *)
   Definition s0_3 := Eval vm_compute in (add_roots (S.make nclauses3) root3 used_roots3).
   Print s0_3.
-  (* s0_3 = ({| [6] |}, 
-    0 :: nil, 4) : PArray.Map.t C.t * C.t * int *)
-  (* 3 := p ^ ~p *)
-
+  (* s0_3 = ({|  |} *)
   Eval vm_compute in List.nth 0 (fst c3) _.
-  (* 1. First step: BuildDef 1 8 *)
+  (* 1. *)
   Definition s1_3 := Eval vm_compute in (step_checker s0_3 (List.nth 0 (fst c3) (CTrue t_func3 t_atom3 t_form3 0))).
   Print s1_3.
-  (* s1_3 = ({| [6],  [2; 7; 8] |}, 
-    0 :: nil, 4) : PArray.Map.t C.t * C.t * int *)
+  (* s1_3 = ({|  |} *)
 
   Eval vm_compute in List.nth 1 (fst c3) _.
-  (* 2. Res 0 {| 1, 0 |} *)
+  (* 2. *)
   Definition s2_3 := Eval vm_compute in (step_checker s1_3 (List.nth 1 (fst c3) (CTrue t_func3 t_atom3 t_form3 0))).
   Print s2_3.
-  (* s1_3 = ({| [2, 8],  [2; 7; 8] |}, 
-    0 :: nil, 4) : PArray.Map.t C.t * C.t * int *)
+  (* s2_3 = ({|  |} *)
 
   Eval vm_compute in List.nth 2 (fst c3) _.
-  (* 3. CFalse 1 *)
+  (* 3. *)
   Definition s3_3 := Eval vm_compute in (step_checker s2_3 (List.nth 2 (fst c3) (CTrue t_func3 t_atom3 t_form3 0))).
   Print s3_3.
-  (* s1_3 = ({| [2, 8],  [3] |}, 
-    0 :: nil, 4) : PArray.Map.t C.t * C.t * int *)
+  (* s3_3 = ({|  |} *)
 
   Eval vm_compute in List.nth 3 (fst c3) _.
-  (* 4. Res 1 {| 0, 1 |} *)
+  (* 4. *)
   Definition s4_3 := Eval vm_compute in (step_checker s3_3 (List.nth 3 (fst c3) (CTrue t_func3 t_atom3 t_form3 0))).
   Print s4_3.
-  (* s1_3 = ({| [2, 8],  [8] |}, 
-    0 :: nil, 4) : PArray.Map.t C.t * C.t * int *)
+  (* s4_3 = ({|  |} *)
 
   Eval vm_compute in List.nth 4 (fst c3) _.
-  (* 5. ImmBuildProj 0 1 0 *)
+  (* 5. *)
   Definition s5_3 := Eval vm_compute in (step_checker s4_3 (List.nth 4 (fst c3) (CTrue t_func3 t_atom3 t_form3 0))).
   Print s5_3.
-  (* s1_3 = ({| [6], [8] |}, 
-    0 :: nil, 4) : PArray.Map.t C.t * C.t * int *)
+  (* s5_3 = ({|  |} *)
 
   Eval vm_compute in List.nth 5 (fst c3) _.
-  (* 6. ImmBuildProj 2 0 0 *)
+  (* 6. *)
   Definition s6_3 := Eval vm_compute in (step_checker s5_3 (List.nth 5 (fst c3) (CTrue t_func3 t_atom3 t_form3 0))).
   Print s6_3.
-  (* s1_3 = ({| [6], [8], [4] |}, 
-    0 :: nil, 4) : PArray.Map.t C.t * C.t * int *)
+  (* s6_3 = ({|  |} *)
 
   Eval vm_compute in List.nth 6 (fst c3) _.
-  (* 7. ImmBuildProj 0 0 1 *)
+  (* 7. *)
   Definition s7_3 := Eval vm_compute in (step_checker s6_3 (List.nth 6 (fst c3) (CTrue t_func3 t_atom3 t_form3 0))).
   Print s7_3.
-  (* s1_3 = ({| [5], [8], [4] |}, 
-    0 :: nil, 4) : PArray.Map.t C.t * C.t * int *)
+  (* s7_3 = ({|  |} *)
 
   Eval vm_compute in List.nth 7 (fst c3) _.
-  (* 8. BuildProj 3 10 0 *)
+  (* 8. *)
   Definition s8_3 := Eval vm_compute in (step_checker s7_3 (List.nth 7 (fst c3) (CTrue t_func3 t_atom3 t_form3 0))).
   Print s8_3.
-  (* s1_3 = ({| [5], [8], [4], [4; 10] |}, 
-    0 :: nil, 4) : PArray.Map.t C.t * C.t * int *)
+  (* s8_3 = ({|  |} *)
 
   Eval vm_compute in List.nth 8 (fst c3) _.
-  (* 9. Res 3 ({| 0, 3 |}) *)
+  (* 9. *)
   Definition s9_3 := Eval vm_compute in (step_checker s8_3 (List.nth 8 (fst c3) (CTrue t_func3 t_atom3 t_form3 0))).
   Print s9_3.
-  (* s1_3 = ({| [5], [8], [4], [10] |}, 
-    0 :: nil, 4) : PArray.Map.t C.t * C.t * int *)
-  
+  (* s9_3 = ({|  |} *)
+
   Eval vm_compute in List.nth 9 (fst c3) _.
-  (* 10. ImmBuildDef 3 3 *)
+  (* 10. *)
   Definition s10_3 := Eval vm_compute in (step_checker s9_3 (List.nth 9 (fst c3) (CTrue t_func3 t_atom3 t_form3 0))).
   Print s10_3.
-  (* s1_3 = ({| [5], [8], [4], [2; 5] |}, 
-    0 :: nil, 4) : PArray.Map.t C.t * C.t * int *)
+  (* s10_3 = ({|  |} *)
 
   Eval vm_compute in List.nth 10 (fst c3) _.
-  (* 11. Res 3 {| 2, 3, |} *)
+  (* 11. *)
   Definition s11_3 := Eval vm_compute in (step_checker s10_3 (List.nth 10 (fst c3) (CTrue t_func3 t_atom3 t_form3 0))).
   Print s11_3.
-  (* s1_3 = ({| [5], [8], [4], [2] |}, 
-    0 :: nil, 4) : PArray.Map.t C.t * C.t * int *)
+  (* s11_3 = ({|  |} *)
 
   Eval vm_compute in List.nth 11 (fst c3) _.
-  (* 12. ImmBuildProj 1 1 1 *)
+  (* 12. *)
   Definition s12_3 := Eval vm_compute in (step_checker s11_3 (List.nth 11 (fst c3) (CTrue t_func3 t_atom3 t_form3 0))).
   Print s12_3.
-  (* s1_3 = ({| [5], [3], [4], [2] |}, 
-    0 :: nil, 4) : PArray.Map.t C.t * C.t * int *)
+  (* s12_3 = ({|  |} *)
 
   Eval vm_compute in List.nth 12 (fst c3) _.
-  (* 12. Res 1 {| 3, 1 |} *)
+  (* 13. *)
   Definition s13_3 := Eval vm_compute in (step_checker s12_3 (List.nth 12 (fst c3) (CTrue t_func3 t_atom3 t_form3 0))).
   Print s13_3.
-  (* s1_3 = ({| [5], [], [4], [2] |}, 
-    0 :: nil, 4) : PArray.Map.t C.t * C.t * int *)
+  (* s13_3 = ({|  |} *)
 
-  (* If the main_checker returns true, SMTCoq has successfully managed to check the proof *)
-  Eval vm_compute in (euf_checker C.is_false (add_roots (S.make nclauses3) root3 used_roots3) c3 conf3).
-End Checker_SmtEx3Debug.
+  Eval vm_compute in List.nth 13 (fst c3) _.
+  (* 14. *)
+  Definition s14_3 := Eval vm_compute in (step_checker s13_3 (List.nth 13 (fst c3) (CTrue t_func3 t_atom3 t_form3 0))).
+  Print s14_3.
+  (* s14_3 = ({|  |} *)
 
-Lemma ex3: forall p, negb (p && (negb p)).
-Proof.
-  verit_bool.
-Qed.
+  Eval vm_compute in List.nth 14 (fst c3) _.
+  (* 15. *)
+  Definition s15_3 := Eval vm_compute in (step_checker s14_3 (List.nth 14 (fst c3) (CTrue t_func3 t_atom3 t_form3 0))).
+  Print s15_3.
+  (* s15_3 = ({|  |} *)
+
+  Eval vm_compute in List.nth 15 (fst c3) _.
+  (* 16. *)
+  Definition s16_3 := Eval vm_compute in (step_checker s15_3 (List.nth 15 (fst c3) (CTrue t_func3 t_atom3 t_form3 0))).
+  Print s16_3.
+  (* s16_3 = ({|  |} *)
+
+  Eval vm_compute in List.nth 16 (fst c3) _.
+  (* 17. *)
+  Definition s17_3 := Eval vm_compute in (step_checker s16_3 (List.nth 16 (fst c3) (CTrue t_func3 t_atom3 t_form3 0))).
+  Print s17_3.
+  (* s17_3 = ({|  |} *)
+
+  Eval vm_compute in List.nth 17 (fst c3) _.
+  (* 18. *)
+  Definition s18_3 := Eval vm_compute in (step_checker s17_3 (List.nth 17 (fst c3) (CTrue t_func3 t_atom3 t_form3 0))).
+  Print s18_3.
+  (* s18_3 = ({|  |} *)
+
+  Eval vm_compute in List.nth 18 (fst c3) _.
+  (* 19. *)
+  Definition s19_3 := Eval vm_compute in (step_checker s18_3 (List.nth 18 (fst c3) (CTrue t_func3 t_atom3 t_form3 0))).
+  Print s19_3.
+  (* s19_3 = ({|  |} *)
+
+  Eval vm_compute in List.nth 19 (fst c3) _.
+  (* 20. *)
+  Definition s20_3 := Eval vm_compute in (step_checker s19_3 (List.nth 19 (fst c3) (CTrue t_func3 t_atom3 t_form3 0))).
+  Print s20_3.
+  (* s20_3 = ({|  |} *)
+
+  Eval vm_compute in List.nth 20 (fst c3) _.
+  (* 21. *)
+  Definition s21_3 := Eval vm_compute in (step_checker s20_3 (List.nth 20 (fst c3) (CTrue t_func3 t_atom3 t_form3 0))).
+  Print s21_3.
+  (* s21_3 = ({|  |} *)
+
+  Eval vm_compute in List.nth 21 (fst c3) _.
+  (* 22. *)
+  Definition s22_3 := Eval vm_compute in (step_checker s21_3 (List.nth 21 (fst c3) (CTrue t_func3 t_atom3 t_form3 0))).
+  Print s22_3.
+  (* s22_3 = ({|  |} *)
+
+  Eval vm_compute in List.nth 22 (fst c3) _.
+  (* 23. *)
+  Definition s23_3 := Eval vm_compute in (step_checker s22_3 (List.nth 22 (fst c3) (CTrue t_func3 t_atom3 t_form3 0))).
+  Print s23_3.
+  (* s23_3 = ({|  |} *)
+
+  Eval vm_compute in List.nth 23 (fst c3) _.
+  (* 24. *)
+  Definition s24_3 := Eval vm_compute in (step_checker s23_3 (List.nth 23 (fst c3) (CTrue t_func3 t_atom3 t_form3 0))).
+  Print s24_3.
+  (* s24_3 = ({|  |} *)
+
+  Eval vm_compute in List.nth 24 (fst c3) _.
+  (* 25. *)
+  Definition s25_3 := Eval vm_compute in (step_checker s24_3 (List.nth 24 (fst c3) (CTrue t_func3 t_atom3 t_form3 0))).
+  Print s25_3.
+  (* s25_3 = ({|  |} *)
+
+  Eval vm_compute in List.nth 25 (fst c3) _.
+  (* 26. *)
+  Definition s26_3 := Eval vm_compute in (step_checker s25_3 (List.nth 25 (fst c3) (CTrue t_func3 t_atom3 t_form3 0))).
+  Print s26_3.
+  (* s26_3 = ({|  |} *)
+
+  Eval vm_compute in List.nth 26 (fst c3) _.
+  (* 27. *)
+  Definition s27_3 := Eval vm_compute in (step_checker s26_3 (List.nth 26 (fst c3) (CTrue t_func3 t_atom3 t_form3 0))).
+  Print s27_3.
+  (* s27_3 = ({|  |} *)
+
+  Eval vm_compute in List.nth 27 (fst c3) _.
+  (* 28. *)
+  Definition s28_3 := Eval vm_compute in (step_checker s27_3 (List.nth 27 (fst c3) (CTrue t_func3 t_atom3 t_form3 0))).
+  Print s28_3.
+  (* s28_3 = ({|  |} *)
+
+  Eval vm_compute in List.nth 28 (fst c3) _.
+  (* 29. *)
+  Definition s29_3 := Eval vm_compute in (step_checker s28_3 (List.nth 28 (fst c3) (CTrue t_func3 t_atom3 t_form3 0))).
+  Print s29_3.
+  (* s29_3 = ({|  |} *)
+
+  Eval vm_compute in List.nth 29 (fst c3) _.
+  (* 30. *)
+  Definition s30_3 := Eval vm_compute in (step_checker s29_3 (List.nth 29 (fst c3) (CTrue t_func3 t_atom3 t_form3 0))).
+  Print s30_3.
+  (* s30_3 = ({|  |} *)
+
+  Eval vm_compute in List.nth 30 (fst c3) _.
+  (* 31. *)
+  Definition s31_3 := Eval vm_compute in (step_checker s30_3 (List.nth 30 (fst c3) (CTrue t_func3 t_atom3 t_form3 0))).
+  Print s31_3.
+  (* s31_3 = ({|  |} *)
+
+  Eval vm_compute in List.nth 31 (fst c3) _.
+  (* 32. *)
+  Definition s32_3 := Eval vm_compute in (step_checker s31_3 (List.nth 31 (fst c3) (CTrue t_func3 t_atom3 t_form3 0))).
+  Print s32_3.
+  (* s32_3 = ({|  |} *)
+
+End Test3Debug.
